switched to autosubst2(ocaml); lemma cong respect lt proved

.CoqMakefile.d
@@ -1,4 +1,0 @@
-theories/CongLtLemma.vo theories/CongLtLemma.glob theories/CongLtLemma.v.beautified theories/CongLtLemma.required_vo: theories/CongLtLemma.v theories/Proc.vo /home/sbf/.opam/autosubst-master/lib/rocq-runtime/rocqworker
-theories/CongLtLemma.vos theories/CongLtLemma.vok theories/CongLtLemma.required_vos: theories/CongLtLemma.v theories/Proc.vos /home/sbf/.opam/autosubst-master/lib/rocq-runtime/rocqworker
-theories/Proc.vo theories/Proc.glob theories/Proc.v.beautified theories/Proc.required_vo: theories/Proc.v /home/sbf/.opam/autosubst-master/lib/rocq-runtime/rocqworker
-theories/Proc.vos theories/Proc.vok theories/Proc.required_vos: theories/Proc.v /home/sbf/.opam/autosubst-master/lib/rocq-runtime/rocqworker
