pi.sig
@@ -1,0 +1,13 @@
+-- Signature for System F
+
+-- the types
+chan : Type
+proc : Type
+
+
+-- Res : (bind chan in proc) -> proc
+-- the constructors for proc
+Zero : proc  
+Par : proc -> proc -> proc 
+Rcv : chan -> (bind chan in proc) -> proc
+Send : chan -> chan -> proc -> proc
