theories/CongLtLemma.v
@@ -1,19 +1,91 @@
 
-Require Import Proc.
+Require Import ProcSyn.
+Require Import Semantics.
+Require Import unscoped.
+Require Import core.
+Import ProcSyn.Core.
+Import unscoped.UnscopedNotations.
+ 
+
+
+ (*  --- a bunch of tactics for replacement in conga and lt hypotheses  ---  *)
+Ltac subinallleft_lt  :=
+ try match goal with
+| [H: lt ?P ?a ?P', Heq: ?ter=?P|- _] => symmetry in Heq; rewrite Heq in *; symmetry in Heq
+end .
+
+  
+Ltac subinallright_lt  :=
+ try match goal with
+| [H: lt ?P ?a ?P', Heq: ?ter=?P'|- _] => symmetry in Heq; rewrite Heq in *; symmetry in Heq
+end .
+
+Ltac subinall_lt := subinallleft_lt; subinallright_lt. 
+
+Ltac subinallleft_conga  :=
+ try match goal with
+| [H: conga ?P ?P', Heq: ?ter=?P|- _] => symmetry in Heq; rewrite Heq in *; symmetry in Heq
+end .
+
+
+Ltac subinallright_conga  :=
+ try match goal with
+| [H: conga ?P ?P', Heq: ?ter=?P'|- _] => symmetry in Heq; rewrite Heq in *; symmetry in Heq
+end .
+
+Ltac subinall_conga := subinallleft_conga; subinallright_conga. 
+
+
+(*note that if terms are nested it won't work*)
+Ltac subinall := subinall_lt ; subinall_conga. 
+(*------------------------------*)
+
+
+
+Lemma conga_resp_sub: forall P Q sigma,
+  conga P Q -> conga (P [sigma]) (Q [sigma]).
+Proof.
+intros.
+inversion H.
+asimpl. eauto with picalc.
+asimpl. eauto with picalc.
+asimpl. eauto with picalc.
+Qed.
+
+Lemma cong_resp_sub: forall P Q sigma,
+  cong P Q -> cong (P [sigma]) (Q [sigma]).
+Proof.
+intros.
+generalize dependent sigma.
+induction H.
+intro.
+set ( D := conga_resp_sub P Q sigma H).
+eauto with picalc.
+eauto with picalc.
+eauto with picalc.
+eauto with picalc.
+asimpl. eauto with picalc.
+asimpl. eauto with picalc.
+asimpl. eauto with picalc.
+
+intro. 
+eapply Cg_ctxRcv.  
+eauto with picalc.
+Qed.
 
 
 
 
-
-
-Lemma conga_resp_lt: forall P Q P' a, 
+  
+ 
+Lemma Lconga_resp_lt: forall P Q P' a, 
   lt P a P'-> conga P Q -> exists Q', lt Q a Q' /\ conga P' Q'.
 Proof.
 intros. 
 inversion H.  (*caseAn on lt derivation*)
 (*======all the cases of Lt_send======*)  
-inversion H0. 
-subinall. 
+inversion H0 .
+subinall.   
 exfalso. inversion H0.
 subinall. 
 exfalso. inversion H0.
@@ -21,7 +93,7 @@ subinall.
 exfalso. inversion H0.
 (* ======all the cases of Lt_rcv======*)
 inversion H0.
-subinall.  
+subinall.   
 exfalso. inversion H0.
 subinall. 
 exfalso. inversion H0.
@@ -30,217 +102,413 @@ exfalso. inversion H0.
 (*======all the cases parL======*)
 inversion H0.
 (*subcase com*)
-subinall.  
+
+
+subinall.     
 inversion H2. (*destroy the AST*)
-rewrite H2 in H0.
-rewrite H2 in H.
-rewrite H9 in H.
-rewrite H8 in H1.
-exists (Par Q1 P'0). split.
-apply (Lt_parR Q1 P1  P'0 a).
-apply H1.
-apply (Cga_parCom P'0 Q1).
+econstructor . split. eapply Lt_parR.  
+symmetry in H8; rewrite H8 in *. eapply H1 .
+intuition .   
 (*subcase assoc*)  
 
-subinall. 
+subinall.  
 inversion H2. (*destruct the AST*)
-rewrite H8 in H1.
+(*rewrite H8 in H1.*)
   (*caseAn on P1|Q1 ->a P'0*)
+  subst.  
   inversion H1.
-  exists (Par P'1 (Par Q1 R)). split.
-  apply (Lt_parL  (Par Q1 R) P1 P'1 a ).
-  apply H13.
-  apply (Cga_parAssoc P'1 Q1 R).
-  
-  exists (Par P1 (Par Q' R)). split.
-  apply (Lt_parR P1 (Par Q1 R) (Par Q' R) a).
-  apply (Lt_parL R Q1 Q' a).
-  apply H13.
-  apply (Cga_parAssoc P1 Q' R).
-  
-  exists ( Par P'1 (Par Q' R) ). split.
-  apply (Lt_commL P1 (Par Q1 R) P'1 (Par Q' R) q r).
-  apply H11. 
-  apply (Lt_parL R Q1 Q' (Lrcv q r)).
-  apply H14.
-  apply (Cga_parAssoc P'1 Q' R). 
+    
+  eexists. split.  
+  eauto with picalc.
+  intuition.
 
-  exists (Par P'1 (Par Q' R)). split.
-  apply (Lt_commR P1 (Par Q1 R) P'1 (Par Q' R) q r).
-  apply H11.
-  apply (Lt_parL  R Q1 Q' (Lsend q r)).
-  apply H14.
-  apply (Cga_parAssoc P'1 Q' R).
+  eexists. split.
+  eauto with picalc.
+  intuition.
+
+  eexists. split.
+  eauto with picalc.
+  intuition.
+
+  eexists. split.
+  eauto with picalc.
+  intuition.
+
 (*subcase neut*)
-  subinall.
-  inversion H2. (*destroy the AST*)
-  rewrite H8 in *.
-  exists (P'0). split.
-  apply H1.
-  apply (Cga_parNeut P'0).
   
+  eexists. split.
+  subst.
+  inversion H5.
+  subst.
+  apply H1.
+  subst. inversion H5.
+  intuition.
+
 (*======all the cases parR======*)
 inversion H0.
 (*subcase com*)
-subinall. 
-inversion H2. (*destroy the AST*)
-symmetry in H9;rewrite H9.
-exists (Par Q' P1). split.
-apply (Lt_parL P1 Q0 Q' a).
-apply H1.
-apply (Cga_parCom P1 Q').
+
+eexists. split.
+subst.
+inversion H5.
+subst.
+eauto with picalc.
+subst. inversion H5. 
+intuition.
+
 (*subcase assoc*)
-subinall.  
+(*subinall.*)  
+
+subst.
 
 (* caseAn on conga*)
 inversion H0.
-
-exists (Par Q' (Par Q1 R)). split.
-rewrite H10 in *.
-apply (Lt_parL (Par Q1 R) P1 Q' a).
-apply H1.
-apply (Cga_parCom (Par Q1 R) Q').
  
-exists (Par P1 (Par Q1 Q')). split.
-rewrite H12 in *.
-apply (Lt_parR P1 (Par Q1 R) (Par Q1 Q') a).
-apply (Lt_parR  Q1 R Q' a).
-apply H1.
-apply (Cga_parAssoc P1 Q1 Q').
+eexists. split.
+subst.
+eapply Lt_parL.
+eapply H1.
+subst.
+intuition. 
 
-subinall. 
-rewrite H7 in *.
+eexists. split.
+subst.
+eapply Lt_parR. eapply Lt_parR.
+eapply H1.
+subst.
+intuition.
+
+subst.
 exfalso. inversion H1.
-
 (*subcase neut*)
-subinall. 
-inversion H2. (*destroy AST*)
-rewrite H9 in *.
-(*caseAn on conga*)
-inversion H0.
+subst.
+inversion H5.
+subst.
 exfalso. inversion H1.
-exfalso. inversion H1.
-exfalso. inversion H1.
-
+ 
 (* ======all the cases of Lt_commL======*)
 inversion H0. (*caseAn on conga*)
+subst. 
+inversion H6. (*destruct AST*) 
+  
+eexists. split.
+eauto with picalc. intuition.
 
-subinall. 
-inversion H3. (*destruct AST*)
-rewrite H9, H10 in *.
-symmetry in H4;rewrite H4 in H.
-exists (Par Q' P'0). split.
-apply (Lt_commR Q1 P1 Q' P'0 q r).
-apply H2. apply H1.
-apply (Cga_parCom P'0 Q').
-
-subinall.
-inversion H3. (*destruct AST*)
-rewrite H9 in *.
-symmetry in H4;rewrite H4 in H.   
-inversion H1.  
-(*caseAn on   P1|Q1 ->(q!r)   P'0*)  
+subst.
+inversion H6.
+symmetry in H4;rewrite H4 in H1.
+inversion H1.  (*caseAn on   P1|Q1 ->(q!r)   P'0*) 
+eexists. split.
+eauto with picalc. intuition.
 (**)
-rewrite H10 in H2. 
-exists (Par P'1 (Par Q1 Q')). split.
-apply (Lt_commL P1 (Par Q1 R) P'1 (Par Q1 Q') q r).
-apply H14.
-apply (Lt_parR Q1 R Q' (Lrcv q r)).
-apply H2.
-apply (Cga_parAssoc P'1 Q1 Q').
-(**)
-rewrite H10  in H2.
-exists (Par P1 (Par Q'0 Q')). split.
-apply (Lt_parR P1 (Par Q1 R) (Par Q'0 Q') Ltau).
-apply (Lt_commL Q1 R Q'0 Q' q r).
-apply H14.
-apply H2.
-apply (Cga_parAssoc P1 Q'0 Q').
+eexists. split.
+eauto with picalc. intuition.
 
-subinall. 
-inversion H3. (*destroy AST*)
-rewrite H10 in *.
+subst. 
+inversion H6. subst.
 exfalso. inversion H2.
+
+
 (* ======all the cases of Lt_commR======*)
 inversion H0.
 
-subinall.
-inversion H3. (*destroy AST*)
-rewrite H9,H10 in *.
-exists (Par Q' P'0). split.
-apply (Lt_commL Q1 P1 Q' P'0 q r).
-apply H2. apply H1.
-apply (Cga_parCom P'0 Q').
+subst.
+eexists. split.
+inversion H6. 
+eauto with picalc. intuition.
+ 
+subst.
+inversion H6.
+symmetry in H4,H5; rewrite H5 in H2; rewrite H4 in H1.
+inversion H1. (*caseAn on   P1|Q1 ->(q?r)   P'0*)
+eexists. split.
+rewrite H5 in *.
+eapply Lt_commR.
+eauto with picalc. eauto with picalc. intuition.
+(**)
+eexists. split.
+subst.
+eapply  Lt_parR.
+eauto with picalc. subst. intuition.
 
-subinall.
-inversion H3. (*destroy AST*)
-subinall.
-rewrite H10 in H2. rewrite H9 in H1.
-(*caseAn on   P1|Q1 ->(q?r)   P'0*)
-inversion H1.
-exists (Par P'1 (Par Q1 Q')). split.
-apply (Lt_commR P1 (Par Q1 R) P'1 (Par Q1 Q') q r).
-apply H14. 
-apply (Lt_parR Q1 R Q' (Lsend q r)). apply H2.
-apply (Cga_parAssoc P'1 Q1 Q').
-(**) 
-exists (Par P1 (Par Q'0 Q')). split.
-apply (Lt_parR P1 (Par Q1 R) (Par Q'0 Q') Ltau).
-apply (Lt_commR Q1 R Q'0 Q' q r).
-apply H14. apply H2.
-apply (Cga_parAssoc P1 Q'0 Q').
-
-subinall. 
-inversion H3. (*destroy AST*)
-rewrite H10 in *.
+subst.
+inversion H6.
+subst.
 exfalso. inversion H2.
 Qed.
 
 
-(*
-    -----------         ----------------------
-    P|0 conga P         (P|Q)|R  conga P|(Q|R)
 
 
-         ---------------
-         P|Q   conga Q|P
-
-*)
-
-(*
-Lemma cong_inv_conga: forall P Q, 
-  conga P Q -> 
-    exists P0, P0 cong 
-*)
 
 
-Hint Constructors lt cong conga: core. 
+Lemma Rconga_resp_lt: forall P Q Q' a, 
+  lt Q a Q'-> conga P Q -> exists P', lt P a P' /\ conga P' Q'.
+Proof.
+intros.  
+inversion H.  (*caseAn on lt derivation*)
+(*======all the cases of Lt_send======*)  
+inversion H0 .
+subst.   
+exfalso.  inversion H5.
+subst. 
+exfalso. inversion H5.
+subst. 
+eauto with picalc.
+(* ======all the cases of Lt_rcv======*)
+inversion H0.
+subst.   
+exfalso. inversion H5.
+subst. 
+exfalso. inversion H5.
+subst.
+eauto with picalc. 
+(*======all the cases parL======*)
+inversion H0.
+(*subcase com*)
 
-Axiom skip: forall A, A.
+ 
+subst.     
+inversion H6. (*destroy the AST*)
+eauto with picalc.
+(*subcase assoc*)  
 
-Lemma cong_resp_lt: forall P P' Q Q' a,  
+subst.  
+inversion H6. (*destruct the AST*)
+(*rewrite H8 in H1.*)
+  (*caseAn on P1|Q1 ->a P'0*)
+  subst.
+  eauto with picalc.  
+(*subcase neut*)
+  subst.
+  eauto with picalc.  
+
+(*======all the cases parR======*)
+inversion H0.
+(*subcase com*)
+
+subst.
+inversion H6. 
+eauto with picalc.
+
+(*subcase assoc*)
+subst.
+inversion H6.
+subst.
+
+inversion H0. (* caseAn on conga*)
+ 
+eexists. split.
+subst.
+eauto with picalc.
+
+subst. 
+eauto with picalc.
+
+subst.
+inversion H1. (*case an on Q1|R ->a ...*)
+eauto with picalc.
+eauto with picalc.
+eauto with picalc.
+eauto with picalc.
+subst. eauto with picalc.
+
+(*subcase neut*)
+subst.
+eauto with picalc. 
+(* ======all the cases of Lt_commL======*)
+inversion H0. (*caseAn on conga*)
+subst.  
+inversion H7. (*destruct AST*) 
+eauto with picalc.
+  
+subst.
+inversion H7.
+symmetry in  H5; rewrite H5 in H2.
+inversion H2. (*caseAn on Q1|R ->a ... *)
+subst.
+eauto with picalc.
+subst.
+eauto with picalc.
+
+subst.
+eauto with picalc.
+
+(* ======all the cases of Lt_commR======*)
+inversion H0.
+
+subst.
+eexists. split.
+inversion H7.
+eauto with picalc. intuition.
+ 
+subst.
+inversion H7.
+symmetry in H5; rewrite H5 in H2.
+inversion H2. (*caseAn on Q1|R ->a ...*)
+eauto with picalc.
+eauto with picalc.
+
+subst.
+eauto with picalc.
+Qed.
+
+
+
+
+
+
+Lemma cong_resp_lt: forall P Q P' Q' a, 
   cong P Q -> 
-   (lt P a P' -> exists Q0, lt Q a Q0 /\ cong P' Q0) /\
-   (lt Q a Q' -> exists P0, lt P a P0 /\ cong P0 Q').
-Proof. 
+     (lt P a P'  -> exists Q0, lt Q a Q0 /\ cong P' Q0)  /\
+      (lt Q a Q' -> exists P0, lt P a P0 /\ cong P0 Q').
+Proof.
 intros. 
 generalize dependent P'.
-generalize dependent Q'. 
-induction H. 
-apply skip.
-apply skip.
+generalize dependent Q'.
+generalize dependent a.
+induction H.
 
-intros. split.
-intro. 
-assert(exists P0 : proc, lt Q a P0 /\ cong P0 Q').
-set (IHr:=IHcong P' P' ).
-destruct IHr.
-set (ex:= H2 H0).
-destruct ex.
-exists x. split.
-destruct H3.
-apply H3.
-destruct H3.
+(*case conga*)
+intros. firstorder.
+assert (exists Q0, lt Q a Q0 /\ conga P' Q0).
+eapply Lconga_resp_lt.
+eauto with picalc. auto.
+firstorder.
+eauto with picalc.
+(**)
+assert( exists P0, lt P a P0 /\ conga P0 Q').
+eapply Rconga_resp_lt.
+eauto with picalc. auto.
+firstorder.
+eauto with picalc.
+(*case refl*)
+
+firstorder.  
+eauto with picalc. 
+eauto with picalc.
+(*case sym*)
+
+firstorder. 
+set (IHdestr := IHcong a P' P'). 
+firstorder. eauto with picalc.
+(**)
+firstorder.
+set (IHdestr := IHcong a Q' Q').
+firstorder .
+eauto with picalc.
+
+(*case trans*)
+firstorder.
+ 
+set (D1:= IHcong1 a P' P').  destruct D1. 
+set (d1 := H2 H1).
+firstorder.
+set(D2 := IHcong2 a x x).
+firstorder.  eauto with picalc.
+(**)
+set (D1:= IHcong2 a Q' P'). destruct D1.
+firstorder.
+set (D2 := IHcong1 a x P'). firstorder. eauto with picalc. 
+(*case parL*)
+firstorder.   
+inversion H0. (*caseAn on P|Q ->a  ...*)
+subst.
+set (D1 := IHcong a Q' P'1 ). 
+firstorder. eauto with picalc. 
+ 
+eauto with picalc.
+
+subst.
+set (D1:= IHcong (Lsend x y) Q' P'1). 
+firstorder. eauto with picalc.
+
+subst.
+set (D1 := IHcong (Lrcv x y) Q' P'1).
+firstorder. eauto with picalc.
+(**)
+inversion H0. (*caseAn on P'|Q ->a  ...*)
+subst.
+set (D1 := IHcong a  P'1 Q). 
+firstorder. eauto with picalc.
+ 
+eauto with picalc.
+ 
+subst.
+set (D1 := IHcong (Lsend x y) P'1 Q ). 
+firstorder. eauto with picalc.
+
+subst.
+set (D1 := IHcong (Lrcv x y) P'1 Q ). 
+firstorder.
+eauto with picalc.
+(*case parR*)
+firstorder.
+inversion H0. (*caseAn on P|Q ->a  ...*)
+
+subst.
+eauto with picalc.
+
+subst.
+set (D1 := IHcong a Q Q'1 ). firstorder.
+eauto with picalc.
+
+subst. 
+set (D1:= IHcong (Lrcv x y) P Q'1). firstorder.
+eauto with picalc.
+
+subst. 
+set (D1 := IHcong (Lsend x y) P Q'1). firstorder.
+eauto with picalc.
+(**)
+inversion H0. (*caseAn on P|Q' ->a  ...*)
+ 
+eauto with picalc. 
+
+subst.
+set (D1:= IHcong a Q'1 P). firstorder.
+eauto with picalc.
+ 
+subst.
+set (D1:= IHcong (Lrcv x y) Q'1 P). firstorder.
+eauto with picalc.
+
+subst.
+set (D1:= IHcong (Lsend x y) Q'1 P). firstorder.
+eauto with picalc.
+
+(*case send*)
+firstorder. 
+inversion H0.
+subst.
+eauto with picalc.
+
+inversion H0.
+subst.
+eauto with picalc.
+
+(*case rcv*)
+firstorder.
+inversion H0.
+subst. 
+eexists. split.
+eauto with picalc.
+
+set (lem := cong_resp_sub P P' (y..)).
+firstorder.
+
+inversion H0.
+subst.
+eexists. split.
+eauto with picalc.
+set (lem := cong_resp_sub P P' (y..)).
+firstorder.
+Qed.
+
+
+
+
+
 
 
 
@@ -248,82 +516,28 @@ destruct H3.
 
 
 (*
-Inductive lt: proc -> lab -> proc -> Prop :=
-| Lt_send: forall Q R P, lt (Send Q R P) (Lsend Q R) P 
-| Lt_rcv: forall Q P q, lt (Rcv Q P) (Lrcv Q q) (P.[q/])
-| Lt_parL: forall Q P P' a, lt P a P' -> lt (Par P Q) a (Par P' Q) 
-| Lt_parR: forall P Q Q' a, lt Q a Q' -> lt (Par P Q) a (Par P Q')
-| Lt_commL: forall P Q P' Q' q r, 
-    lt P (Lsend q r) P' -> lt Q (Lrcv q r) Q' -> lt (Par P Q) Ltau (Par P' Q')
-| Lt_commR: forall P Q P' Q' q r, 
-    lt P (Lrcv q r) P' -> lt Q (Lsend q r) Q' -> lt (Par P Q) Ltau (Par P' Q')
-.
-
-
-(*   (proc, |)  commutative monoid up to conga *)
-Inductive conga: proc -> proc -> Prop :=
-| Cga_parCom: forall P Q,     conga (Par P Q)  (Par Q P)
-| Cga_parAssoc: forall P Q R, conga (Par (Par P Q) R)    (Par P (Par Q R))
-| Cga_parNeut: forall P,      conga (Par P Zero) P
-.
-
-(*  cong = conga + equivrel + ctxrules *)
-Inductive cong: proc -> proc -> Prop :=
-| Cg_cga: forall P Q,     conga P Q -> cong P Q
-| Cg_refl: forall P,       cong P P
-| Cg_sym: forall P Q,     cong Q P -> cong P Q
-| Cg_trans: forall P Q R, cong P Q -> cong Q R -> cong P R
-| Cg_ctxParL: forall P P' Q, cong P P' -> cong (Par P Q) (Par P' Q)  
-| Cg_ctxParR: forall P Q Q', cong Q Q' -> cong (Par P Q) (Par P Q')
-| Cg_ctxSend: forall Q R P P', cong P P' -> cong (Send Q R P) (Send Q R P')
-| Cg_ctxRcv: forall Q P P', cong P P' -> cong (Rcv Q P) (Rcv Q P')
-.
-*)
-
-
-
-
-(*
-
-
-
-Lemma cong_resp_lt: forall P P' a, forall Q,  
-  cong P Q->  lt P a P' -> exists Q', lt Q a Q' /\ cong P' Q'.
-Proof. 
+Lemma Testcong_resp_lt: forall P Q P' Q' a, 
+  cong P Q -> 
+     (lt P a P'  -> exists Q0, lt Q a Q0 /\ cong P' Q0)  /\
+      (lt Q a Q' -> exists P0, lt P a P0 /\ cong P0 Q').
+Proof.
 intros.
 induction H. 
-(*===basecase conga===*)
-
-assert (exists Q0 : proc, lt Q a Q0 /\ conga P' Q0).
-apply (conga_resp_lt P Q P' a). apply H0. apply H.
-destruct H1.  
-exists x. destruct H1. split. apply H1. apply (Cg_cga P' x). apply H2.
-(*===basecase refl===*)
-
-exists P'. split. 
-apply H0. apply (Cg_refl P').
-(*===indcase sym===*)
-
-
-
-
-
-
-
-
-
-
-attempt with ind on P->a P'
-intros. generalize dependent Q.
-induction H. 
-
-(*===base case Lt_send===*)
-intros.   
-inversion H0. (*caseAn on Q!R.P cong Q0   *)
- 
-exfalso. inversion H.
-
-exists P. split.
-apply (Lt_send Q R P). apply (Cg_refl P).
+(*case conga*)
+firstorder.
+set (leml := Lconga_resp_lt P Q P' a H0 H).
+destruct leml.
+firstorder. 
+eauto with picalc.
+(**)
+set (lemr := Rconga_resp_lt P Q Q' a H0 H).
+destruct lemr. firstorder. 
+eauto with picalc.
+(*case refl*)
+firstorder.  
+eauto with picalc.
+eauto with picalc.
+(*case sym*)
+firstorder.
 
 *)
