Makefile
@@ -7,7 +7,7 @@
 ##         #     GNU Lesser General Public License Version 2.1          ##
 ##         #     (see LICENSE file for the text of the license)         ##
 ##########################################################################
-## GNUMakefile for Rocq 9.1+alpha
+## GNUMakefile for Rocq 9.0.0
 
 # For debugging purposes (must stay here, don't move below)
 INITIAL_VARS := $(.VARIABLES)
@@ -48,7 +48,7 @@ CoqMakefile.conf: _CoqProject
 	rocq makefile -f _CoqProject -o CoqMakefile
 
 # This file can be created by the user to hook into double colon rules or
-# add any other Makefile code they may need
+# add any other Makefile code he may need
 -include CoqMakefile.local
 
 # Parameters ##################################################################
@@ -77,6 +77,7 @@ TIMED?=
 TIMECMD?=
 # Use command time on linux, gtime on Mac OS
 TIMEFMT?="$(if $(findstring undefined, $(flavor 1)),$@,$(1)) (real: %e, user: %U, sys: %S, mem: %M ko)"
+ifneq (,$(TIMED))
 ifeq (0,$(shell command time -f "" true >/dev/null 2>/dev/null; echo $$?))
 STDTIME?=command time -f $(TIMEFMT)
 else
@@ -85,6 +86,9 @@ STDTIME?=gtime -f $(TIMEFMT)
 else
 STDTIME?=command time
 endif
+endif
+else
+STDTIME?=command time -f $(TIMEFMT)
 endif
 
 COQBIN?=
@@ -274,7 +278,7 @@ COQDOCLIBS?=$(COQLIBS_NOML)
 # generated this makefile
 # NB --print-version is not in the rocq shim
 COQ_VERSION:=$(shell $(ROCQ) c --print-version | cut -d " " -f 1)
-COQMAKEFILE_VERSION:=9.1+alpha
+COQMAKEFILE_VERSION:=9.0.0
 
 # COQ_SRC_SUBDIRS is for user-overriding, usually to add
 # `user-contrib/Foo` to the includes, we keep COQCORE_SRC_SUBDIRS for
@@ -678,8 +682,8 @@ clean::
 	$(HIDE)rm -f $(VOFILES)
 	$(HIDE)rm -f $(VOFILES:.vo=.vos)
 	$(HIDE)rm -f $(VOFILES:.vo=.vok)
-	$(HIDE)rm -f $(VOFILES:.vo=.vo.prof.json)
-	$(HIDE)rm -f $(VOFILES:.vo=.vo.prof.json.gz)
+	$(HIDE)rm -f $(VOFILES:.vo=.v.prof.json)
+	$(HIDE)rm -f $(VOFILES:.vo=.v.prof.json.gz)
 	$(HIDE)rm -f $(BEAUTYFILES) $(VFILES:=.old)
 	$(HIDE)rm -f all.ps all-gal.ps all.pdf all-gal.pdf all.glob all-mli.tex
 	$(HIDE)rm -f $(VFILES:.v=.glob)
